src/Common/Literal.v
@@ -1,4 +1,4 @@
-From Utils Require Import Int.
+From Utils Require Import Int Tactics.
 
 Inductive literal : Set := 
 | IntLit (n: int) 
@@ -12,3 +12,9 @@ Definition lit_eqb l1 l2 :=
   | UnitLit, UnitLit => true
   | _, _ => false
   end.
+
+Lemma lit_eqb_refl : forall l, lit_eqb l l = true.
+Proof.
+  destruct l; simpl;
+  auto using Z.eqb_refl, Bool.eqb_reflx.
+Qed.
